Major work on alpha equivalence. Definitions, lemmas, WIP SN proof. Contains lots of old definitions.

src/PlutusIR/Semantics/Static/normaliser/SN_STLC_named.v
@@ -1,5 +1,3 @@
-(** * Strong Normalization of System F *)
-
 From mathcomp Require Import ssreflect ssrbool eqtype ssrnat.
 From Coq Require Import ssrfun.
 Require Import Coq.Strings.String.
@@ -15,91 +13,8 @@ Set Implicit Arguments.
 Unset Strict Implicit.
 Unset Printing Implicit Defensive.
 From PlutusCert Require Import STLC_named STLC_named_typing ARS.
+From PlutusCert Require Import alpha.
 
-
-(** **** Capms lemmas *)
-(*
-
-TODO: alternatief
-Jacco:
-Het is misschien wat makkelijker om Equations te gebruiken in ipv Program Fixpoint, equations is wat uitgebreider en meer onderhouden (https://github.com/mattam82/Coq-Equations?tab=readme-ov-file#documentation)
-GitHub - mattam82/Coq-Equations: A function definition package for Coq
-A function definition package for Coq. Contribute to mattam82/Coq-Equations development by creating an account on GitHub.
- 
-die genereert de unfold lemmas sowieso
- 
-al die lemmas komen dan in een hintdb genaamd capms, die je dan met autorewrite with capms kan gebruiken.
- 
-dat is dan je alternatief voor wat je bij een niet-recursieve functie zou doen met simpl
- *)
-Lemma capms_var sigma X t:
-  lookup X sigma = Some t -> capms sigma (tmvar X) = t.
-Proof. 
-  rewrite capms_equation_1. 
-  by move=> ->. (* TODO: this is copilot stuff, I dont understand that*)
-Qed.
-
-Lemma capms_lam X B sigma s :
-  capms sigma (tmlam X B s) = 
-    tmlam (fresh2 sigma s) B (capms sigma (rename X (fresh2 sigma s) s)).
-Proof.
-  rewrite capms_equation_2.
-  reflexivity.
-Qed.
-
-(** **** Notations *)
-(* Notation for substitution *)
-Notation "'[' x ':=' s ']' t" := (capms [(x, s)] t) (at level 20).
-
-Notation "sigma [[ t ]]" := (capms sigma t) (at level 20).
-
-(** **** One-Step Reduction *)
-
-(* Set Implicit Arguments.
-Unset Strict Implicit.
-Unset Printing Implicit Defensive.
-
-Delimit Scope prop_scope with PROP.
-Open Scope prop_scope. *)
-
-(* Alpha reduction based on Andrej Bauer (Computer Science stack exchange)*)
-(* Inductive relation for:
-
-equalVar :: [(Var,Var)] -> Var -> Var -> Bool
-equalVar [] x y = (x == y)
-equalVar ((x,y):bound) z w = (x == z && y == w) || (x /= z && y /= w && equalVar bound z w)
-
-equal' :: [(Var, Var)] -> Term -> Term -> Bool
-equal' bound (Belong x1 y1) (Belong x2 y2) = (equalVar bound x1 x2 && equalVar bound y1 y2)
-equal' bound Bot Bot = True
-equal' bound (Imply u1 v1) (Imply u2 v2) = equal' bound u1 u2 && equal' bound v1 v2
-equal' bound (Forall x u) (Forall y v) = equal' ((x,y):bound) u v
-equal' _ _ _ = False
-
-*)
-Inductive AlphaVar : list (string * string) -> string -> string -> Prop :=
-| alpha_var_refl x : AlphaVar [] x x
-| alpha_var_cons x y z w sigma :
-    x = z ->
-    y = w ->
-    AlphaVar ((x, y) :: sigma) z w
-| alpha_var_diff x y z w sigma :
-    x <> z -> 
-    y <> w -> 
-    AlphaVar sigma z w -> 
-    AlphaVar ((x, y) :: sigma) z w.
-
-Inductive Alpha : list (string * string) -> term -> term -> Prop :=
-| alpha_var x y sigma : 
-    AlphaVar sigma x y -> 
-    Alpha sigma (tmvar x) (tmvar y)
-| alpha_lam x y A s1 s2 sigma :
-    Alpha ((x, y) :: sigma) s1 s2 -> 
-    Alpha sigma (tmlam x A s1) (tmlam y A s2)
-| alpha_app s1 s2 t1 t2 sigma :
-    Alpha sigma s1 s2 -> 
-    Alpha sigma t1 t2 -> 
-    Alpha sigma (tmapp s1 t1) (tmapp s2 t2).
 
 (* Contextual alpha equivalence: kinding contexts that match alpha contexts*)
 Inductive CAlpha : list (string * string) -> list (string * type) -> list (string * type) -> Prop :=
@@ -167,7 +82,14 @@ Proof.
     apply K_App with (K1 := K1); assumption.
 Qed.
 
-Inductive step : term -> term -> Prop :=
+
+(* ********************
+      Beta reduction
+*)
+
+
+(* TODO: Used to be Prop. Ask Jacco*)
+Inductive step : term -> term -> Set :=
 | step_beta (x : string) (A : type) (s t : term) :
     step (tmapp (tmlam x A s) t) ([x := t] s)
 | step_appL s1 s2 t :
@@ -181,77 +103,923 @@ Lemma step_ebeta x A s t u :
   u = ([x := t] s) -> step (tmapp (tmlam x A s) t) u.
 Proof. move->. exact: step_beta. Qed.
 
-(* See Barendregt 1984*)
-
-(* Ask Richard's pen and paper notes*)
-Lemma capmsRename x x' t sigma s :
-  ((x', t)::sigma) [[rename x x' s]] = ((x, t)::sigma) [[s]].
-Proof. 
-Admitted.
-
-Definition notKeyIn X (sigma : list (string * term)) : Prop :=
-  ~ exists t, lookup X sigma = Some t.
-
-Definition varNotIn X (sigma : list (string * term)) : Prop :=
-  notKeyIn X sigma /\ (* X does not appear in the free type variables of any of the values  of tau*)
-  ~ In X (List.flat_map (compose ftv snd) sigma).
-
-(* Definitionally, 
-  fresh2 creates a fresh variable that is not in 
-    any of the keys or values of sigma *)
-Lemma freshLemma sigma s :
-  varNotIn (fresh2 sigma s) sigma.
-Proof. Admitted.
-
-(* TODO: why cant i use list syntax?*)
-Lemma composeCapms' X t X' t' s :
-  varNotIn X [(X', t')] -> [X := t] ([X' := t'] s) = ((X, t):: cons (X', t') nil) [[s]].
-Proof.
-  intros HnotIn.
-  (* Induction on s?*)
-Admitted.
-
-(* Would also work for bigger substs, but not necessary*)
-Lemma composeCapms X t sigma s :
-  varNotIn X sigma -> [X := t] (sigma [[s]]) = ((X, t) :: sigma) [[s]].
-Proof.
-Admitted.
-
-(*
-  But what if sigma contains x.
-  Then RHS will replace this by sigma(x)
-  while LHS will replace it by t.
-*)
-Lemma commute_subst s t sigma x :
-  sigma [[ [x := t] s]] = ((x, sigma [[t]])::sigma) [[s]].
-Proof.
-Admitted.
-
-(* Stepping does not change free vars*)
-Lemma step_preserves_fresh_sigma s t1 t2 x : step t1 t2 -> fresh2 [(x, t1)] s = fresh2 [(x, t2)] s.
-Proof.
-Admitted.
-
+(* This is not true ... *)
 Lemma step_preserves_fresh sigma t1 t2 : 
   step t1 t2 -> fresh2 sigma t1 = fresh2 sigma t2.
 Proof.
 Admitted.
-
 (* TODO: Not true because of fresh, what conditions do we need? *)
 (* e.g. rename X Y (tmlam Y A (tmvar X)) = tmlam Y A (tmvar Y). 
   that case shouldnt be possible. But Y is not in ftv (tmlam Y A (tmvar X))
   should we consider all type variables, not only the free ones for ftv?
 
 *)
-Lemma ren_is_subst : forall X X' s,
-  rename X X' s = [X := tmvar X'] s.
-Proof.
-Abort.
 
-(* TODO: some conditions necessary like X'  not in sigma*)
-Lemma ren_sub_compose : forall sigma X X' s,
-  sigma [[rename X X' s]] = ((X, tmvar X')::sigma) [[s]].
+Lemma de_morgan2 : forall P Q : Prop, ~ (P \/ Q) <-> ~ P /\ ~ Q.
 Proof.
+  intros P Q. split.
+  - intros H. split.
+    + intros HP. apply H. left. assumption.
+    + intros HQ. apply H. right. assumption.
+  - intros [H1 H2] [HP | HQ].
+    + apply H1. assumption.
+    + apply H2. assumption.
+Qed.
+
+(* For the var case we needed to also alpha t,x,y to make it consistent with ren*)
+Lemma ren_sub_compose''_var_fix x x' y y' s t ren ren1 ren2 s' s'':
+  AlphaCtxTrans ren1 ren2 ren -> 
+  Alpha ren1 s' s -> 
+  Alpha ren2 s s'' -> 
+  Alpha ren t t -> (* this condition is saying x not in t implicitly if (x,y) in ren????? *)
+  AlphaVar ren x y ->
+  AlphaVar ren x' y' ->
+
+  ~ In x' (tv ([x := t] s')) -> (* TODO: I dont want this condition! It is saying like x' is " super"  fresh: 
+    x' is not equal to any of the fresh variables generated in the subst operation*)
+  Alpha ren (rename x x' ([x := t] s')) ([y := rename y y' t] s'').
+Proof.
+  (* destruct (in_dec (String.string_dec) y (tv t)).
+  {
+  generalize dependent s'.
+  generalize dependent s''.
+  generalize dependent ren1.
+  generalize dependent ren2.
+  generalize dependent ren.
+  induction s; intros ren ren2 ren1 s'' s' Htrans Halphas1 Halphas2 Halphat Hmrenx Hmrenx' Hx'Fresh.
+  - inversion Halphas1.
+    inversion Halphas2.
+    subst.
+    rewrite capms_equation_1.
+    simpl.
+    destr_eqb_eq x x0.
+    + (* Since x = x0, we should always have y = y1*)
+      assert (AlphaVar ren x0 y1) by admit.
+      destr_eqb_eq y y1.
+      * rewrite capms_equation_1.
+        simpl.
+        rewrite String.eqb_refl.
+        
+        
+        
+        (*
+          Then we are renaming alpha (under ren) terms to alpha (under ren) terms in a term that is alpha (under ren).
+          Should be ok?
+        *)
+        admit.
+      * (* contradiction somewhere 
+        
+          Some lemma that converts    
+              mren ren (tmvar x0) = tmvar y 
+          to
+              AlphaVar ren x0 y
+
+          Then we have
+            AlphaVar ren x0 y
+            AlphaVar ren x0 y1
+
+          That is only possible if y = y1.
+        *)
+        admit.
+    + 
+      (*
+        By mren ren (tmvar x) = tmvar y
+          then
+        AlphaVar ren x y
+
+        By 
+          x <> x0
+          AlphaVar ren x0 y1
+          AlphaVar ren x y
+        
+        Then:
+          y <> y1
+        (because otherwise AlphaVar ren x0 y1 and AlphaVar ren x y1, not possible with x0 <> x)
+        *)
+      destr_eqb_eq y y1.
+      * admit. (* by above not possible: contradiction*)
+      * rewrite capms_equation_1.
+        simpl.
+        destr_eqb_eq y y1.
+        -- contradiction.
+        -- unfold rename. unfold mren.
+           simpl.
+           destr_eqb_eq x x0.
+           ++ contradiction.
+           ++ apply alpha_var.
+              admit. (* by alpha_trans*)
+  - (* Case: Lam *)
+    inversion Halphas1.
+    inversion Halphas2.
+    rewrite capms_equation_2.
+    rewrite capms_equation_2.
+    simpl.
+    subst.
+    remember (fresh2 [(x, t)] s1) as s0'.
+    remember (fresh2 [(y, rename y y' t)] s4) as s0''.
+    destr_eqb_eq x s0'.
+    + (* contradiction fresh s0' *)
+      admit.
+    + unfold rename.
+      unfold mren. fold mren.
+      
+      assert (Hdrop: drop s0' [(x, x')] = ((x, x')::nil)) by admit.
+      rewrite Hdrop.
+      apply alpha_lam.
+
+      assert (Alpha [(s0', x0)] (rename x0 s0' s1) s1).
+      {
+        apply @alpha_sym with (ren := ((x0, s0')::nil)).
+        - apply alpha_sym_cons.
+          apply alpha_sym_nil.
+        - apply alphaRename.
+          (* s0' notin tv s1 follows from s0' = fresh2 [(x, t)] s1*)
+          admit.
+      }
+      assert (HtransRes1: Alpha ((s0', s)::ren1) (rename x0 s0' s1) s0).
+      {
+        remember (ctx_id_left ren1) as ren_id.
+
+        (* by transitivity and H2: Alpha ((x0, s) :: ren1) s1 s0*)
+        apply @alpha_trans with (ren := (s0', x0)::ren_id ) (ren' := (x0, s)::ren1) (t := s1).
+        - apply alpha_trans_cons.
+          rewrite Heqren_id.
+          apply id_left_trans.
+        - 
+          assert ((s0', x0)::ren_id = ((s0', x0)::nil) ++ ren_id) by reflexivity.
+          rewrite H1.
+          apply alpha_extend_ids_right.
+          + rewrite Heqren_id.
+            apply ctx_id_left_is_id.
+          + assumption.
+        - assumption.
+      }
+
+      (* ANALOGOUS*)
+      assert (Alpha ((s, y1) :: ren2) s0 s4) by assumption. (* By assumption: This is saying that in s4, we already have s replaced by y0!*)
+      assert (Alpha [(y1, s0'')] s4 (rename y1 s0'' s4)) by admit.
+      assert (HtransRes2: Alpha ((s, s0'')::ren2) s0 (rename y1 s0'' s4)) by admit. (* Transitivity. then here we replace y0 by s0'', since s4 already has s replaced by y0, we dont have to change the replace arguments*)
+
+      assert (Htrans': AlphaCtxTrans ((s0', s)::ren1) ((s, s0'')::ren2) ((s0', s0'')::ren)) by admit.
+      
+      specialize (IHs ((s0', s0'')::ren) ((s, s0'')::ren2) ((s0', s)::ren1) (rename y1 s0'' s4) (rename x0 s0' s1) Htrans').
+      specialize (IHs HtransRes1 HtransRes2).
+      
+      assert (HalphatExtend : Alpha ((s0', s0'')::ren) t t) by admit. (* s0' and s0'' fresh over t!*)
+
+      (* here we use that x' is not equal to any of the fresh variables generated by [x := t] (such as s0')*)
+      assert (Hx'FreshExtendAndHnots0'x' : s0' <> x' /\ ~ (In x' (tv ([x := t] (rename x0 s0' s1))))).
+      {
+        rewrite capms_equation_2 in Hx'Fresh.
+        simpl in Hx'Fresh.
+        rewrite <- Heqs0' in Hx'Fresh.
+        (* rewrite not or*)
+        rewrite -> de_morgan2 in Hx'Fresh.
+        destruct Hx'Fresh as [Hnots0'x' Hx'Fresh].
+        split; assumption.
+      }
+      
+      destruct Hx'FreshExtendAndHnots0'x' as [Hnots0'x' Hx'FreshExtend].
+
+      specialize (IHs HalphatExtend).
+
+      assert (HAlphaVarXExtend: AlphaVar ((s0', s0'') :: ren) x y) by admit. (* x, y fresh under s0', s0''*)
+
+      assert (y' <> s0'') by admit. (* By y in tv t and s0'' = fresh2 [(y, rename y y' t)]: TODO: We probably need ftv instead of tv*)
+
+      assert (HAlphaVarYExtend: AlphaVar ((s0', s0'') :: ren) x' y') by admit.
+
+      specialize (IHs HAlphaVarXExtend HAlphaVarYExtend Hx'FreshExtend).
+
+      apply IHs.
+  - admit.
+  }
+  {
+    (* y notin tv t, by AlphaVar ren x y, we have [(x, y)] in ren
+      hence not x in t.
+     *)
+    assert (rename y y' t = t) by admit.
+    rewrite H.
+    intros Htrans HalphaS1 HalphaS2 Halphat HalphaVarx HalphaVarx' Hx'Fresh.
+    clear Hx'Fresh.
+    clear HalphaVarx'.
+    generalize dependent s'.
+    generalize dependent s''.
+    generalize dependent ren.
+    generalize dependent ren1.
+    generalize dependent ren2.
+    induction s; intros ren2 ren1 ren Htrans Halphat HalphaVarx s'' HalphaS1 s' HalphaS2.
+    - admit.
+    - intros.
+      inversion HalphaS1.
+      subst.
+      inversion HalphaS2.
+      subst.
+      rewrite capms_equation_2.
+      rewrite capms_equation_2.
+      simpl.
+      remember (fresh2 [(x, t)] s1) as s0'.
+      remember (fresh2 [(y, t)] s2) as s0''.
+      assert (Hxs0': x <> s0') by admit.
+      assert (HrenLam: rename x x' (tmlam s0' t0 ([x := t] rename x0 s0' s1)) = tmlam s0' t0 (rename x x' ([x := t] (rename x0 s0' s1)))) by admit.
+      rewrite HrenLam.
+      apply alpha_lam.
+      
+
+      assert (Alpha [(s0', x0)] (rename x0 s0' s1) s1).
+      {
+        apply @alpha_sym with (ren := ((x0, s0')::nil)).
+        - apply alpha_sym_cons.
+          apply alpha_sym_nil.
+        - apply alphaRename.
+          (* s0' notin tv s1 follows from s0' = fresh2 [(x, t)] s1*)
+          admit.
+      }
+      assert (HtransRes1: Alpha ((s0', s)::ren1) (rename x0 s0' s1) s0).
+      {
+        remember (ctx_id_left ren1) as ren_id.
+
+        (* by transitivity and H2: Alpha ((x0, s) :: ren1) s1 s0*)
+        apply @alpha_trans with (ren := (s0', x0)::ren_id ) (ren' := (x0, s)::ren1) (t := s1).
+        - apply alpha_trans_cons.
+          rewrite Heqren_id.
+          apply id_left_trans.
+        - 
+          assert ((s0', x0)::ren_id = ((s0', x0)::nil) ++ ren_id) by reflexivity.
+          rewrite H1.
+          apply alpha_extend_ids_right.
+          + rewrite Heqren_id.
+            apply ctx_id_left_is_id.
+          + assumption.
+        - assumption.
+      }
+
+      (* ANALOGOUS*)
+      assert (Alpha ((s, y0) :: ren2) s0 s2) by assumption. (* By assumption: This is saying that in s4, we already have s replaced by y0!*)
+      assert (Alpha [(y0, s0'')] s2 (rename y0 s0'' s2)) by admit.
+      assert (HtransRes2: Alpha ((s, s0'')::ren2) s0 (rename y0 s0'' s2)) by admit. (* Transitivity. then here we replace y0 by s0'', since s4 already has s replaced by y0, we dont have to change the replace arguments*)
+
+      assert (Htrans': AlphaCtxTrans ((s0', s)::ren1) ((s, s0'')::ren2) ((s0', s0'')::ren)) by admit.
+      
+      specialize (IHs  ((s, s0'')::ren2) ((s0', s)::ren1) ((s0', s0'')::ren) Htrans').
+      
+      assert (HalphatExtend : Alpha ((s0', s0'')::ren) t t) by admit. (* s0' and s0'' fresh over t!*)
+
+      assert (HalphaVarxExtend : AlphaVar ((s0', s0'') :: ren) x y) by admit.
+
+      specialize (IHs HalphatExtend HalphaVarxExtend (rename y0 s0'' s2) HtransRes2).
+
+      specialize (IHs (rename x0 s0' s1) HtransRes1).
+
+      apply IHs.
+    - admit.
+  } *)
+Admitted.
+
+Lemma ren_lam_vacuous x x' t s0 :
+  rename x x' (tmlam x t s0) = tmlam x t s0.
+Proof.
+  unfold rename.
+  simpl. rewrite String.eqb_refl. rewrite mren_id. reflexivity.
+Qed.
+
+Lemma ren_lam x x' t s s0 :
+  x <> s -> rename x x' (tmlam s t s0) = tmlam s t (rename x x' s0).
+Proof.
+  intros Hnotxs.
+  unfold rename.
+  simpl. rewrite <- String.eqb_neq in Hnotxs. rewrite Hnotxs.
+  reflexivity.
+Qed.
+
+Lemma ren_commute x x' y y' s :
+  x <> y ->
+  x' <> y ->
+  y' <> x ->
+  rename x x' (rename y y' s) = rename y y' (rename x x' s).
+Proof.
+  intros Hxy Hx'y Hy'x.
+  induction s.
+  - simpl.
+    destr_eqb_eq y s.
+    + destr_eqb_eq x s.
+      * contradiction.
+      * unfold rename.
+        simpl. rewrite String.eqb_refl. rewrite <- String.eqb_neq in H. rewrite H. simpl.
+        rewrite <- String.eqb_neq in Hy'x. rewrite String.eqb_sym in Hy'x. rewrite Hy'x.
+        rewrite String.eqb_refl.
+        reflexivity.
+    + unfold rename. simpl. rewrite <- String.eqb_neq in H. rewrite H.
+      destr_eqb_eq x s.
+      * simpl. rewrite String.eqb_refl. rewrite <- String.eqb_neq in Hx'y. rewrite String.eqb_sym in Hx'y. rewrite Hx'y.
+        reflexivity.
+      * simpl. rewrite <- String.eqb_neq in H0. rewrite H0. rewrite H.
+        reflexivity.   
+  - destr_eqb_eq y s.
+    + rewrite ren_lam_vacuous.
+      rewrite ren_lam; [|assumption].
+      rewrite ren_lam_vacuous.
+      reflexivity.
+    + destr_eqb_eq x s.
+      * rewrite ren_lam_vacuous;
+        rewrite ren_lam; [|assumption].
+        rewrite ren_lam_vacuous; reflexivity.
+      * rewrite ren_lam; [|assumption].
+        rewrite ren_lam; [|assumption].
+        rewrite ren_lam; [|assumption].
+        rewrite ren_lam; [|assumption].
+        rewrite IHs.
+        reflexivity.
+  - unfold rename. simpl.
+    unfold rename in IHs1.
+    unfold rename in IHs2.
+    rewrite IHs1.
+    rewrite IHs2.
+    reflexivity.
+Qed.
+
+Lemma ren_two_vacuous {x Y' Y s }:
+  x <> Y ->
+  rename x Y' (rename x Y s) = rename x Y s.
+Proof.
+
+Admitted.
+
+Lemma ren_vacuous X Y s :
+  ~ In X (tv s) -> rename X Y s = s.
+Proof.
+Admitted.
+
+Lemma sub_vacuous_stronger X t Y u Y' s s' s'' ren ren1 ren2 :
+  AlphaVar ren Y Y' ->
+  Alpha ren u u ->
+  AlphaCtxTrans ren1 ren2 ren ->
+  ren1 ⊢ s' ~ s ->
+  ren2 ⊢ s ~ s'' ->
+  ~ In X (tv s') -> Alpha ren (((X, t)::(Y, u)::nil) [[ s' ]]) (((Y', u)::nil) [[ s'' ]]).
+Proof.
+  intros HalphaY HalphaU HalphaTrans Halphas1 Halphas2 Hnotins.
+  generalize dependent ren.
+  generalize dependent ren1.
+  generalize dependent ren2.
+  generalize dependent s'.
+  generalize dependent s''.
+  induction s; intros s'' s' HxnotIns' ren2 Halphas2 ren1 Halphas1 ren HalphaY HalphaU HalphaTrans.
+  - inversion Halphas1.
+    inversion Halphas2.
+    subst.
+    rewrite capms_equation_1.
+    simpl.
+    destr_eqb_eq X x.
+    + unfold tv in HxnotIns'.
+      rewrite not_in_cons in HxnotIns'.
+      destruct HxnotIns'.
+      contradiction.
+    + (* X <> x *)
+            assert (AlphaVar ren x y0).
+        {
+          eapply alpha_var_trans; eauto.
+        }
+      destr_eqb_eq Y x.
+      * 
+
+        assert (y0 = Y').
+        {
+          eapply alphavar_unique; eauto.
+        }
+        rewrite H1.
+        rewrite capms_equation_1.
+        simpl.
+        rewrite String.eqb_refl.
+        assumption.
+      * (* AlphaVar x y0
+          x <> Y and AlphaVar Y Y'. Therefore y0 <> Y'
+      *)
+        remember H0 as H0_copy.
+        clear HeqH0_copy.
+        apply (alphavar_unique_not H1 HalphaY) in H0.
+        rewrite capms_equation_1.
+        simpl.
+        rewrite <- String.eqb_neq in H0.
+        rewrite H0.
+        apply alpha_var.
+        assumption.
+
+
+
+      (* By AlphaVar ren x y0 and AlphaVar ren x Y' => Y' = y0, then by capms_equation-1 we have ren |- u ~ u, assumption*) 
+  - (* By X notin tv (tmlam s t0 s0),   also X notin tv s0, so we can use IHS*)
+    inversion Halphas1.
+    inversion Halphas2.
+    subst.
+    rewrite capms_equation_2.
+    rewrite capms_equation_2.
+    simpl.
+    remember (fresh2 ((x, tmvar x) :: (X, t) :: (Y, u)::nil) s1) as s0'.
+    remember (fresh2 ((y0, tmvar y0) :: (Y', u) :: nil) s4) as s0''.
+
+    apply alpha_lam.
+    eapply IHs.
+    + (* X is not s0' by fresh2. and X is not s1 by X notin tv (tmlam x t0 s1)*)
+      shelve.
+    + eapply @alpha_trans with (ren' := ((y0, s0'')::(ctx_id_right ren2))).
+      * apply alpha_trans_cons.
+          apply id_right_trans.
+      * exact H10.
+      * change ((y0, s0''):: (ctx_id_right ren2)) with (((y0, s0'')::nil) ++ (ctx_id_right ren2)). 
+          apply alpha_extend_ids_right.    
+          -- apply ctx_id_right_is_id.
+          -- apply alphaRename. shelve. (* True by s0'' = fresh2 s4*)
+    + eapply @alpha_trans with (ren := (s0', x) :: (ctx_id_left ren1)).
+      * apply alpha_trans_cons.
+        apply id_left_trans.
+      *  
+        change ((s0', x) :: (ctx_id_left ren1)) with (((s0', x)::nil) ++ (ctx_id_left ren1)).
+        apply alpha_extend_ids_right.
+        -- apply ctx_id_left_is_id.
+        -- eapply alpha_sym.
+          ++ apply alpha_sym_cons. apply alpha_sym_nil.
+          ++ apply alphaRename. shelve.
+      * exact H2.
+    + shelve. (* By fresh2 *)
+    + shelve. (* By fresh2 *)  
+    + apply alpha_trans_cons.
+      exact HalphaTrans.
+  - inversion Halphas1.
+    inversion Halphas2.
+    subst.
+    rewrite capms_equation_3.
+    rewrite capms_equation_3.
+    apply alpha_app.
+    + eapply IHs1.
+      * shelve.
+      * exact H8.
+      * exact H3.
+      * exact HalphaY.
+      * exact HalphaU.
+      * exact HalphaTrans.
+Admitted.
+
+(* Need alpha because the bigger vacuous substitution is used in fresh variable generation *)
+Lemma sub_vacuous X t Y u s :
+  ~ In X (tv s) -> Alpha [] (((X, t)::(Y, u)::nil) [[ s ]]) (((Y, u)::nil) [[ s ]]).
+Proof.
+  intros Hnotins.
+  eapply sub_vacuous_stronger; try constructor; try apply alpha_refl; try constructor.
+  - assumption.
+Qed.
+
+
+(* Is the above still useful? Yes! *)
+Lemma ren_sub_compose''_specific x x' s t :
+  ~ In x' (tv ([x := t] s)) -> Alpha [] (rename x x' ([x := t] s)) ([x := rename x x' t] s). 
+Proof.
+  intros Hfresh.
+  eapply ren_sub_compose''_var_fix; eauto;
+  try constructor;
+  apply alpha_refl;
+  constructor.
+Qed.
+
+Lemma sub_preserves_alpha Z Z' t s s' s'' ren1 ren2 ren :
+  AlphaVar ren Z Z' ->
+  AlphaCtxTrans ren1 ren2 ren ->
+  ren1 ⊢ s' ~ s ->
+  ren2 ⊢ s ~ s'' ->
+  Alpha ren t t ->
+  Alpha ren ([Z := t] s') ([Z' := t] s'').
+Proof.
+  intros HalphaZ HalphaS HalphaT.
+  generalize dependent s'.
+  generalize dependent s''.
+  generalize dependent ren1.
+  generalize dependent ren2.
+  generalize dependent ren.
+  induction s; intros ren HalphaZ ren2 ren1 HalphaTrans s'' s' Halphas1 Halphas2 Halphat.
+  - inversion Halphas1.
+    inversion Halphas2.
+    subst.
+    rewrite capms_equation_1.
+    rewrite capms_equation_1.
+    simpl.
+          assert (AlphaVar ren x y0).
+      {
+        eapply alpha_var_trans; eauto. 
+      }
+    destr_eqb_eq Z x.
+    + (* Z = x, but AlphaVar ren x Z' and AlphaVar ren x y0, so Z' = y0*)
+
+      assert (HZ'y0: Z' = y0). { eapply alphavar_unique; eauto. }
+      rewrite HZ'y0.
+      rewrite String.eqb_refl.
+      assumption.
+    + (* Z <> x*)
+      destruct (Z' =? y0) eqn:HZ'y0.
+      * apply String.eqb_eq in HZ'y0.
+        (* Then AlphaVar ren x y0   and  AlphaVar ren Z y0     then also *)
+        subst.
+        exfalso.
+        apply (alphavar_unique_not H0 HalphaZ) in H.
+        contradiction.
+      * apply alpha_var.
+        assumption. 
+
+  - inversion Halphas1.
+    inversion Halphas2.
+    subst.
+    rewrite capms_equation_2.
+    rewrite capms_equation_2.
+    simpl.
+    remember (fresh2 [(x, tmvar x); (Z, t)] s1) as s0'.
+    remember (fresh2 [(y0, tmvar y0); (Z', t)] s4) as s0''.
+    apply alpha_lam.
+    eapply IHs.
+    + shelve. (* By fresh2 on Z and Z'*)
+    + apply alpha_trans_cons.
+      exact HalphaTrans.
+    + eapply @alpha_trans with (ren := (s0', x) :: (ctx_id_left ren1)).
+      * apply alpha_trans_cons.
+        apply id_left_trans.
+      *  
+        change ((s0', x) :: (ctx_id_left ren1)) with (((s0', x)::nil) ++ (ctx_id_left ren1)).
+        apply alpha_extend_ids_right.
+        -- apply ctx_id_left_is_id.
+        -- eapply alpha_sym.
+          ++ apply alpha_sym_cons. apply alpha_sym_nil.
+          ++ apply alphaRename. shelve.
+      * exact H2.
+    + eapply alpha_trans.
+      * apply alpha_trans_cons.
+          apply id_right_trans.
+      * exact H10.
+      * change ((y0, s0''):: (ctx_id_right ren2)) with (((y0, s0'')::nil) ++ (ctx_id_right ren2)). 
+          apply alpha_extend_ids_right.    
+          -- apply ctx_id_right_is_id.
+          -- apply alphaRename. shelve. (* True by s0'' = fresh2 s4*)
+    + shelve. (* By fresh2 *)
+  - admit. 
+
+Admitted.
+
+Lemma ren_sub_compose_stronger_single : forall s s' s'' ren ren1 ren2 Z Z' t X X' Y,
+  AlphaCtxTrans ren1 ren2 ren ->
+  ren1 ⊢ s' ~ s ->
+  ren2 ⊢ s ~ s'' ->
+  ren ⊢ t ~ t ->
+  AlphaVar ren X X'->
+  (* AlphaVar ren Y Y' ->  IDEA: Remove this whole condition! Y is "superfresh", so it is not changed by ren is the idea! *)
+  AlphaVar ren Y Y ->
+  AlphaVar ren Z Z' ->
+  (* We can add condition X contained (strings) in Y (some freshness condition) *)
+  ~ In Y (tv ([Z := t] s') ++ (Z::nil) ++ (tv s')) -> (* First condition needed for IH, second for var case. 
+    Maybe we need here rename X Y s' instead of s'. That sounds circular, but maybe it is not! *)
+  (* X string contained in Y: *)
+  lt (String.length X) (String.length Y) ->
+  ren ⊢ [Z := t] (rename X Y s') ~ ((X', tmvar Y)::(Z', t)::nil) [[s'']].
+Proof. 
+  intros s s' s'' ren ren1 ren2 Z Z' t X X' Y Htrans HalphaS1 HalphaS2 Halphat HalphaX HalphaY HalphaZ HYfresh Hlength.
+
+
+
+  generalize dependent s'.
+  generalize dependent s''.
+  generalize dependent ren.
+  generalize dependent ren1.
+  generalize dependent ren2.
+
+  induction s; intros ren2 ren1 ren HalphaTrans Halphat HalphaVarX HalphaVarY HalphaVarZ s'' Halphas2 s' Halphas1 HYfresh.
+  - inversion Halphas1.
+    inversion Halphas2.
+    subst.
+    assert (AlphaVar ren x y0). {eapply alpha_var_trans; eauto. }
+    destr_eqb_eq x X.
+    + (* x = X, but alphaVar ren X y0, so alphaVar ren x y0. But AlphaVar ren X X', so y0 = X'*)
+      unfold rename. unfold mren. simpl. rewrite String.eqb_refl.
+      assert (Hy0X': y0 = X'). { eapply alphavar_unique; eauto. }
+      rewrite capms_equation_1.
+      simpl.
+      rewrite not_in_app in HYfresh.
+      destruct HYfresh as [_ HYfresh].
+      rewrite not_in_cons in HYfresh.
+      destruct HYfresh as [HYfresh _].   (* Here we use that Z <> Y*)
+      destr_eqb_eq Z Y.
+      * contradiction.
+      * rewrite Hy0X'.
+        rewrite capms_equation_1. simpl. rewrite String.eqb_refl.
+
+        apply alpha_var.
+        assumption.
+    + (* x <> X*)
+      unfold rename. unfold mren. simpl. rewrite <- String.eqb_neq in H0. assert (X =? x = (x =? X)) by apply String.eqb_sym.
+      rewrite <- H1 in H0. rewrite H0.
+      (* x <> X, but x ~ y0 and X ~ X', so y0 <> X'*)
+      assert (HnotX'y0: X' <> y0). { eapply alphavar_unique_not; eauto. apply String.eqb_neq in H0. assumption. }
+      rewrite capms_equation_1. simpl.
+      rewrite capms_equation_1. simpl.
+      rewrite <- String.eqb_neq in HnotX'y0. rewrite HnotX'y0.
+      destr_eqb_eq Z x.
+      * (* Z = x, but AlphaVar ren x Z' and AlphaVar ren x y0, so Z' = y0*)
+        assert (HZ'y0: Z' = y0). { eapply alphavar_unique; eauto. }
+        rewrite HZ'y0.
+        rewrite String.eqb_refl.
+        assumption.
+      * (* By same logic now Z' <> y0*)
+        assert (HnotZ'y0: Z' <> y0). { eapply alphavar_unique_not; eauto. }
+        rewrite <- String.eqb_neq in HnotZ'y0. rewrite HnotZ'y0.
+        apply alpha_var.
+        assumption.     
+
+  - inversion Halphas1.
+    inversion Halphas2.
+    subst.
+    destr_eqb_eq X x.
+    + assert (HlamRen: rename x Y (tmlam x t0 s1) = tmlam x t0 s1). { unfold rename. unfold mren. fold mren. simpl. rewrite String.eqb_refl. rewrite mren_id. reflexivity. }
+      rewrite HlamRen.
+      rewrite capms_equation_2. (* This should also make it fresh in x I think! *)
+      rewrite capms_equation_2.
+      simpl.
+      remember (fresh2 [(x, tmvar x); (Z, t)] s1) as s0'.
+      remember (fresh2 [(y0, tmvar y0); (X', tmvar Y); (Z', t)] s4) as s0''.
+      apply alpha_lam.
+      assert (Hnotxs0': x <> s0'). { rewrite Heqs0'. shelve. }
+      assert (HrenameVacuous: rename x s0' s1 = rename x Y (rename x s0' s1)). { now rewrite (ren_two_vacuous Hnotxs0'). }
+      rewrite HrenameVacuous.
+
+      assert (Htvlam: tv ([Z := t] (tmlam x t0 s1)) = tv (tmlam s0' t0 ([Z := t] (rename x s0' s1)))).
+        {
+          rewrite capms_equation_2. simpl.
+          rewrite <- Heqs0'.
+          reflexivity.
+        }
+
+      eapply IHs.
+      * apply alpha_trans_cons. exact HalphaTrans.
+      * shelve. (* s0' and s0'' not in t by fresh2.*)
+      * shelve. (* x <> s0' by assumption and X' <> s0'' by fresh2*) 
+      * rewrite Htvlam in HYfresh.
+
+         rewrite not_in_cons in HYfresh.  destruct HYfresh as [HYfresh HYfresh2]; simpl. fold tv in HYfresh2. 
+         apply alpha_var_diff.
+         -- auto.
+         -- shelve. (* By s0'' = fresh2 Y'*)
+         -- assumption.
+      * shelve. (* By fresh2 *)
+      * eapply alpha_trans.
+        -- apply alpha_trans_cons.
+           apply id_right_trans.
+        -- exact H10.
+        -- change ((y0, s0''):: (ctx_id_right ren2)) with (((y0, s0'')::nil) ++ (ctx_id_right ren2)). 
+           apply alpha_extend_ids_right.    
+           ++ apply ctx_id_right_is_id.
+           ++ apply alphaRename. shelve. (* True by s0'' = fresh2 s4*)
+      * eapply @alpha_trans with (ren := (s0', x) :: (ctx_id_left ren1)).
+        -- apply alpha_trans_cons.
+           apply id_left_trans.
+        --  
+           change ((s0', x) :: (ctx_id_left ren1)) with (((s0', x)::nil) ++ (ctx_id_left ren1)).
+            apply alpha_extend_ids_right.
+            ++ apply ctx_id_left_is_id.
+            ++ eapply alpha_sym.
+              ** apply alpha_sym_cons. apply alpha_sym_nil.
+              ** apply alphaRename. shelve. 
+        -- assumption.
+      * rewrite Htvlam in HYfresh.
+        rewrite not_in_cons in HYfresh. destruct HYfresh as [HYfresh HYfresh2]. fold tv in HYfresh2. clear IHs.
+        rewrite not_in_app in HYfresh2.
+        destruct HYfresh2 as [HYfresh2 HYfresh3].
+        rewrite not_in_app.
+        split.
+        -- assumption.
+        -- rewrite not_in_app in HYfresh3. destruct HYfresh3 as [HYfresh3 HYfresh4]; rewrite not_in_app; split.
+           ++ assumption.
+           ++ admit. (* Not in s1 and not equal to s0', hence not in tv (rename x s0' s1)
+           *)
+
+      
+      
+
+    + (* x <> X*) 
+      rewrite ren_lam; [|assumption].
+      rewrite capms_equation_2.
+      rewrite capms_equation_2.
+      simpl.
+      remember (fresh2 [(x, tmvar x); (Z, t)] (rename X Y s1)) as s0'.
+      remember (fresh2 [(y0, tmvar y0);(X', tmvar Y); (Z', t)] s4) as s0''.
+      apply alpha_lam.
+
+      (* Ok, we seem to have to switch out renamings?
+      
+      We know x <> X, so I think this is allowed, if Y = x, we have a problem. Similarly if s0' = X.
+      Y <> x ? yes, by HYfresh
+      s0' = X? Suppose it is. Then no X in (rename X Y s1). Then rename x X s1 yields something with X,
+       and then that gets renamed to Y.
+      We dont want it to be. ??? This can only happen if X=s0' not in t and X <> Z. 
+
+      We know X <> Y (we should add it as a condition!)
+      *)
+      destruct (X =? s0').
+      * assert (Hxs0': X = s0') by shelve. rewrite Hxs0'.
+        (* Maybe we can differentiatie on X in (tmlam x to s1)
+          If it is not in there, there is no renaming. Done! 
+
+          If it is in there, it is in tv (tmlam x t0 s1).
+          Then it is in tv (s1) since x <> X
+          Since X in s1, then Y in rename X Y s1.
+          s0' is then fresh2 over Y.
+
+          But we should have some information somewhere that Y is fresh2 over X.
+
+          Hence s0' cannot be X!
+        *)
+        
+        destruct (in_dec String.string_dec X (tv s1)).
+        -- assert (HYins1: In Y (tv (rename X Y s1))) by shelve.
+           assert (Hlengths0': gt (String.length s0') (String.length Y)) by shelve.
+           rewrite Hxs0' in Hlength.
+           exfalso.
+           lia.
+        -- rewrite ren_vacuous in Heqs0'; [|assumption].
+           assert (HrenVac: rename s0' Y s1 = s1). { rewrite ren_vacuous. - reflexivity. - rewrite Hxs0' in n. assumption. }
+           rewrite HrenVac.
+           (*
+              X not in s1, so X' not in s4 by s1 ~ s4. Also X' <> s0'', hence X' not in rename y0 s0'' s4
+
+           *)
+           assert (HnotX': Alpha [] (((X', tmvar Y):: (Z', t)::nil) [[rename y0 s0'' s4]])  (([Z' := t] (rename y0 s0'' s4)))).
+           {
+            assert (~ In X' (tv (rename y0 s0'' s4))).
+            {
+              (*Alpha ren s1 s4. And X not in s1. So X' not in s4.
+                
+                Then by X' <> s0'': done.
+              *)
+              admit.
+            }
+            eapply sub_vacuous in H0.
+            exact H0.
+           }
+           eapply @alpha_trans with (ren' := (ctx_id_right ((s0'', s0'')::ren))).
+           ++ apply alpha_trans_cons.
+              apply id_right_trans.
+           ++ 
+
+          (* If x is  in s1 then y0 is in s4
+            s0' ~ s0'', s1 ~ s4, Z ~ Z' t ~ t,   all under (s0', s0'')::ren
+
+            So we can use sub_preserves_alpha
+           *)
+           {
+            eapply sub_preserves_alpha.
+            - shelve. (* fresh2 *)
+            - apply alpha_trans_cons. exact HalphaTrans.
+            - eapply @alpha_trans with (ren := (s0', x) :: (ctx_id_left ren1)).
+              + apply alpha_trans_cons.
+                apply id_left_trans.
+              +  
+                change ((s0', x) :: (ctx_id_left ren1)) with (((s0', x)::nil) ++ (ctx_id_left ren1)).
+                  apply alpha_extend_ids_right.
+                  * apply ctx_id_left_is_id.
+                  * eapply alpha_sym.
+                    -- apply alpha_sym_cons. apply alpha_sym_nil.
+                    -- apply alphaRename. shelve.
+              + exact H2.  
+        
+            - eapply alpha_trans.
+              + apply alpha_trans_cons.
+                apply id_right_trans.
+              + exact H10.
+              + change ((y0, s0''):: (ctx_id_right ren2)) with (((y0, s0'')::nil) ++ (ctx_id_right ren2)). 
+                apply alpha_extend_ids_right.    
+                * apply ctx_id_right_is_id.
+                * apply alphaRename. shelve. (* True by s0'' = fresh2 s4*)
+            - shelve. (* fresh2 thing *) 
+           }    
+
+
+           ++ change ((ctx_id_right ((s0'', s0'')::ren))) with (nil++  (ctx_id_right ((s0'', s0'')::ren))).
+              apply alpha_extend_ids_right.    
+              ** apply ctx_id_right_is_id.
+              ** apply @alpha_sym with (ren := nil) (ren' := nil) in HnotX'.
+                 exact HnotX'.
+                 apply alpha_sym_nil.
+
+                   
+           
+
+      * assert (Hnotxs0': X <> s0') by shelve.
+        rewrite ren_commute; try auto; [|shelve]. (* Y <> x by HYfresh*)
+        eapply IHs.
+        -- apply alpha_trans_cons. exact HalphaTrans.
+        -- shelve. (* s0' and s0'' not in t by fresh2.*)
+        -- shelve. (* x <> s0' by assumption and X' <> s0'' by fresh2*)
+        -- rewrite not_in_app in HYfresh. destruct HYfresh as [HYfresh _].
+           rewrite capms_equation_2 in HYfresh. simpl in HYfresh.
+           rewrite de_morgan2 in HYfresh. destruct HYfresh as [HYfresh _].
+           assert (HnotYs0': Y <> s0').
+           {
+              destruct (in_dec String.string_dec X (tv s1)).
+              - assert (HXY: X <> Y) by shelve. (* Fresh condition, X in s1 *)
+                assert (HYins1: In Y (tv (rename X Y s1))) by shelve.
+                shelve. (* Then by freshness condition of Heqs0'*)
+
+
+              - rewrite ren_vacuous in Heqs0'.
+                + rewrite <- Heqs0' in HYfresh. symmetry. assumption.
+                + assumption.
+           }
+           apply alpha_var_diff.
+           ++ auto.
+           ++ shelve. (* By s0'' = fresh2 Y'*)
+           ++ assumption. 
+        -- shelve.
+      -- eapply alpha_trans.
+        ++ apply alpha_trans_cons.
+           apply id_right_trans.
+        ++ exact H10.
+        ++ change ((y0, s0''):: (ctx_id_right ren2)) with (((y0, s0'')::nil) ++ (ctx_id_right ren2)). 
+           apply alpha_extend_ids_right.    
+           ** apply ctx_id_right_is_id.
+           ** apply alphaRename. shelve. (* True by s0'' = fresh2 s4*)
+      -- eapply @alpha_trans with (ren := (s0', x) :: (ctx_id_left ren1)).
+        ++ apply alpha_trans_cons.
+           apply id_left_trans.
+        ++  
+           change ((s0', x) :: (ctx_id_left ren1)) with (((s0', x)::nil) ++ (ctx_id_left ren1)).
+            apply alpha_extend_ids_right.
+            ** apply ctx_id_left_is_id.
+            ** eapply alpha_sym.
+              --- apply alpha_sym_cons. apply alpha_sym_nil.
+              --- apply alphaRename. shelve. (* s0' not in rename X Y s1, and also X <> s0' *) 
+        ++ assumption.
+      -- clear IHs.
+                 (* Y not in tv [z := t] rename x (fresh2 x Z t s1) s1 by assumption.
+                 Also Y <> s0' ?? *)
+
+        rewrite not_in_app in HYfresh. destruct HYfresh as [HYfresh HYfreshlam].
+           rewrite capms_equation_2 in HYfresh. simpl in HYfresh.
+           rewrite de_morgan2 in HYfresh. destruct HYfresh as [HYfresh HYfresh2]. (* Not strong enough I think*)
+           assert (HnotYs0': Y <> s0').
+           {
+              destruct (in_dec String.string_dec X (tv s1)).
+              - assert (HXY: X <> Y) by shelve. (* Fresh condition, X in s1 *)
+                assert (HYins1: In Y (tv (rename X Y s1))) by shelve.
+                shelve. (* Then by freshness condition of Heqs0'*)
+
+
+              - rewrite ren_vacuous in Heqs0'.
+                + rewrite <- Heqs0' in HYfresh. symmetry. assumption.
+                + assumption.
+           }
+           admit. (* HORRIBLE! *)
+                 
+        (*
+        tv (rename x s0' s1) <= tv s0' + tv s1, and it is not equal to any of those, except how to know we dont have to check x?
+
+        *)
+      
+       (* first solve the admit for Y <> s0'*)
+       - admit. 
+  
+
+Admitted.
+
+Lemma fresh_lemma_4 Y X Z t s:
+  Y = (fresh2 ((X, tmvar X)::(Z, t)::nil) s) ->
+  ~ In Y (tv ([Z := t] s)).
+Proof.
+  (* What if s = /X.X
+    tv (/X. f(X)) > tv f(X) ???
+  then [Z:=t] /X. X = /X'. [Z := t] (rename X X' X) where X' = fresh2 [(X, tmvar X); (Z, t)] X , so yes, not equal!
+   *)
+Admitted.
+
+Lemma ren_sub_compose_instantiated X Y Z s t :
+  Y = (fresh2 ((X, tmvar X)::(Z, t)::nil) s) ->
+  nil ⊢ [Z := t] (rename X Y s) ~ ((X, tmvar Y)::(Z, t)::nil) [[s]].
+Proof.
+  intros HYfresh.
+  (* 
+    From HYfresh we can conclude: 
+    When we have a term [Z := t] (tmlam x A s) we create a fresh var exactly equal to Y.
+    and we know Y not in s, Y not in Z, Y not ini t
+    
+    ~ (In Y (tv ([Z := t] s))). ???
+    and therefore 
+  *)
+  eapply ren_sub_compose_stronger_single; eauto; try constructor.
+  - apply alpha_refl. constructor.
+  - apply alpha_refl. constructor.
+  - apply alpha_refl. constructor.
+  - apply not_in_app. split.
+    + now apply fresh_lemma_4 with (X := X).
+    + apply not_in_app. split.
+      * shelve. (* Some fresh property *)
+      * shelve. (* Some fresh property *)   
+Admitted.     
+
+
+
+
   (* This is not exactly true, since rename does not create fresh vars and stuff
         But it is "kind of true" , lol.
 
@@ -262,55 +1030,146 @@ Proof.
         But it should be true, the fact that x' is fresh is key. that will mean that
         capms and rename should behave the same in the tylam case
         SO: TODO: We have to change capms to not freshen if not necessary
+
+        Will it work with alpha equivalence??? Let's work it out on pen and paper
       *)
-      
+Lemma ren_sub_compose : forall sigma x x' s,
+  varNotIn x' sigma ->
+
+  nil ⊢ sigma [[rename x x' s]] ~ ((x, tmvar x')::sigma) [[s]].
+Proof.
+  intros sigma X X' s Hfresh.
+  generalize dependent sigma.
+  induction s; intros sigma Hfresh.
+  - admit.
+  - destr_eqb_eq X s.
+    + admit.
+    + assert (HlamRename: rename X X' (tmlam s t s0) = tmlam s t (rename X X' s0)) by admit.
+      rewrite HlamRename.
+      rewrite capms_equation_2.
+      rewrite capms_equation_2.
+      simpl.
+      remember (fresh2 ((s, tmvar s)::sigma) (rename X X' s0)) as s0'.
+      remember (fresh2 ((s, tmvar s)::(X, tmvar X')::sigma) s0) as s0''.
+      apply alpha_lam.
+      (* Problem! What if s0' = X*)
+      (* IH not strong enough. Need to include alpha contexts and alpha equivalence of s *)
 Admitted.
 
-(* Note: Study: After replacing a variable with something in sigma
-  we can still do the same step as we previously could by red s t, hence: true
-  Not true in non-deterministic setting.
-*)
 
-Lemma step_subst s t : 
-  step s t -> forall sigma, step (sigma [[ s ]]) (sigma [[ t ]]).
+(* We need condition X' not in sigma! 
+   Also X' not in s *)
+Lemma merge_subst : forall sigma X X' s t,
+  nil ⊢ ([X' := t] (((X, tmvar X')::sigma) [[s]])) ~ ((X, t)::sigma) [[s]].
 Proof.
-  move => h.
-  induction h; intros sigma.
+Admitted.
+
+
+
+(* Why do we need this up to alpha equivalence?
+
+  Because sub lemmas are up to alpha equivalence.
+
+  Let's first prove it as an exercise in alpha equivalence proofs and then show its necessity.
+*)
+Lemma step_subst {s t} : 
+  step s t -> forall sigma : list (string * term), {alphaSigmaT : term & 
+  prod (step (sigma [[ s ]]) alphaSigmaT) (Alpha [] alphaSigmaT (sigma [[t]]))} .
+Proof.
+  intros Hstep. induction Hstep; intros sigma.
   - rewrite capms_equation_3.
-    rewrite capms_equation_2.
-    simpl.
-    remember (fresh2 sigma s) as x'.
-    apply step_ebeta.
-    rewrite -> composeCapms.
-    + rewrite -> capmsRename.
-      rewrite commute_subst.
-      reflexivity.
-    + rewrite Heqx'.
-      apply freshLemma.
-  - rewrite capms_equation_3.
-    rewrite capms_equation_3.
-    apply step_appL.
-    specialize (IHh sigma).
-    assumption.
-  - rewrite capms_equation_3.
-    rewrite capms_equation_3.
-    apply step_appR.
-    specialize (IHh sigma).
-    assumption.
-  - rewrite capms_equation_2.
-    rewrite capms_equation_2.
-    simpl.
-    rewrite (step_preserves_fresh sigma h).
-    remember (fresh2 sigma s2) as x'.
-    apply step_abs.
-    rewrite ren_sub_compose.
-    rewrite ren_sub_compose.
-    apply IHh.
+    rewrite capms_equation_2. simpl.
+    remember (fresh2 ((x, tmvar x)::sigma) s) as x'.
+    eexists.
+    split.
+    + eapply step_beta.
+    + 
+    (* exists (((x', sigma [[t]])::nil) [[sigma [[rename x x' s]] ]]). *)
+    (* split. *)
+    + apply step_ebeta. reflexivity.
+    + admit.
+    (* rewrite ren_sub_compose. *)
+        (* rewrite merge_subst.
+        rewrite commute_subst.
+        apply alpha_refl.
+        apply alpha_refl_nil. *)
+  - (* Left application *)
+    specialize (IHHstep sigma).
+    destruct IHHstep as [alphaSigmaS2  [Hs2Step Hs2Alpha]  ].
+    exists (tmapp (alphaSigmaS2) (sigma [[t]])).
+    split.
+    + rewrite capms_equation_3.
+      apply step_appL.
+      assumption.
+    + rewrite capms_equation_3.
+      apply alpha_app.
+      * assumption.
+      * apply alpha_refl.
+        apply alpha_refl_nil.
+  - (* Right applicaiton *)
+    specialize (IHHstep sigma).
+    destruct IHHstep as [alphaSigmaT2  [Ht2Step Ht2Alpha] ].
+    exists (tmapp (sigma [[s]]) alphaSigmaT2).
+    split.
+    + rewrite capms_equation_3.
+      apply step_appR.
+      assumption.
+    + rewrite capms_equation_3.
+      apply alpha_app.
+      * apply alpha_refl.
+        apply alpha_refl_nil.
+      * assumption.
+  - remember (fresh2 ((x, tmvar x)::sigma) s1) as x'.
+    specialize (IHHstep ((x, tmvar x')::sigma)).
+    destruct IHHstep as [alphaSigmaS2  [Hs2Step Hs2Alpha]  ].
+    eexists.
+    (* exists (tmlam x' A alphaSigmaS2). *)
+    split. 
+    + rewrite capms_equation_2. simpl.
+      rewrite <- Heqx'.
+      apply step_abs.
+      (* By ren_sub_compose we know 
+        sigma [[rename x x' s1]] ~ ((x, tmvar x')::sigma) [[s1]]
+
+        Then by alpha_preserves_beta we know
+        exists ?s2 s.t. sigma [[rename x x' s1]] steps to ?s2 and ?s2 ~ alphaSigmaS2 ~ (x, tmvar x'):: sigma [[s2]]
+      *)
+      admit.
+      (* rewrite ren_sub_compose.
+      * assumption.
+      * admit. *)
+    + rewrite capms_equation_2. simpl.
+      assert (Hfresh: (fresh2 sigma s1) = (fresh2 sigma s2)) by apply: step_preserves_fresh Hstep.
+      
+      (* rewrite <- Hfresh. *)
+      (* rewrite <- Heqx'. *)
+      apply alpha_lam.
+      admit.
+      (* rewrite ren_sub_compose.
+      * apply alpha_extend_id'.
+        assumption.
+        apply not_break_shadow_nil.
+      * admit. *)
+Admitted.
+
+
+Lemma step_subst_sigma sigma {s t} :
+  step s t -> {alphaSigmaT : term & prod (step (sigma [[ s ]]) alphaSigmaT) (Alpha [] alphaSigmaT (sigma [[t]]))}.
+Proof.
+  intros Hstep.
+  apply step_subst.
+  assumption.
 Qed.
 
-(** **** Many-Step Reduction *)
+Inductive star {e : term -> term -> Set } (x : term) : term -> Set :=
+| starR : star x x
+| starSE y z : star x y -> e y z -> star x z.
 
-Definition red := star step.
+
+(** **** Many-Step Reduction *)
+Definition red := @star step.
+
+
 
 (* Definition sred sigma tau :=
   forall x : var, red (sigma x) (tau x). *)
@@ -318,18 +1177,40 @@ Definition red := star step.
 Lemma red_app s1 s2 t1 t2 :
   red s1 s2 -> red t1 t2 -> red (tmapp s1 t1) (tmapp s2 t2).
 Proof.
-  move=> A B. apply: (star_trans (tmapp s2 t1)).
+  (* move=> A B. apply: (star_trans (tmapp s2 t1)).
   - apply: (star_hom (tmapp^~ t1)) A => x y. exact: step_appL.
-  - apply: star_hom B => x y. exact: step_appR.
-Qed.
+  - apply: star_hom B => x y. exact: step_appR. *)
+(* Qed. *)
+Admitted.
 
 Lemma red_abs x A s1 s2 : 
   red s1 s2 -> red (tmlam x A s1) (tmlam x A s2).
-Proof. apply: star_hom => x' y'. exact: step_abs. Qed.
+(* Proof. apply: star_hom => x' y'. exact: step_abs. Qed. *)
+Proof. Admitted.
 
-Lemma red_subst sigma s t : 
-  red s t -> red (sigma [[s]]) (sigma [[t]]).
-Proof. apply: star_hom => x' y'. intros Hstep. exact: step_subst. Qed.
+(* TODO: Probably need to prove this with strenghtened induction (non-empty context) for the lambda case *)
+Lemma step_preserves_alpha_nd {s} {s'} {t} :
+  Alpha [] s t -> step s s' -> {t' & prod (step t t') (Alpha [] s' t')}.
+Proof.
+  (* Non-determinism, so only existence, not for all t'*)
+Admitted.
+
+Lemma red_subst sigma {s} {t} : 
+  red s t -> {alphaSigmaT : term & prod (red (sigma [[s]]) alphaSigmaT) (Alpha [] alphaSigmaT (sigma [[t]]))}.
+Proof. 
+  intros Hred.
+  induction Hred. 
+  - exists (sigma [[s]]). split.
+    + apply starR.
+    + apply alpha_refl. constructor.
+  - 
+    apply (step_subst_sigma sigma) in e.
+    
+    destruct IHHred as [alphaSigmaY [Hred' Halpha] ].
+    destruct e as [alphaSigmaZ [Hstep HalphaZ] ].
+    eexists.
+    admit. (* Doable with some alpha arguments*)
+Admitted.
 
 (* Lemma sred_up sigma tau : 
   sred sigma tau -> sred (up sigma) (up tau).
@@ -364,8 +1245,49 @@ Proof.
   (* TODO: Figure out on pen and paper first.*)
 Admitted.
 
+
+
+Lemma rename_preserves_step x x' s t : 
+step s t -> step (rename x x' s) (rename x x' t).
+Proof.
+  intros Hstep.
+  induction Hstep.
+  - destruct (x =? x0) eqn:xx0.
+    + 
+      assert (x = x0) by admit.
+      subst.
+      unfold rename.
+      unfold mren. fold mren.
+      assert (drop x0 [(x0, x')] = nil) by admit.
+      rewrite H.
+      rewrite mren_id.
+      (* Since all x0 in s are replaced by t, we must turn the rhs into
+        rename x0 x' [x0 := rename x0 x' t] s, exactly like lhs
+      *)  
+      assert (mren [(x0, x')] ([x0 := t] s) = [x0 := mren [(x0, x')] t] s) by admit.
+      rewrite H0.
+      apply step_beta.
+
+    + 
+    unfold rename.
+    unfold mren. fold mren.
+    assert (drop x0 [(x, x')] = ((x, x')::nil)) by admit.
+    rewrite H.
+
+    (* Bulk of the work: This is a special case of commute subst! *)
+    assert (mren [(x, x')] ([x0 := t] s) = [x0 := mren [(x, x')] t] (mren [(x, x')] s)) by admit.
+    rewrite H0.
+    apply step_beta.
+  - apply step_appL.
+    assumption.
+  - apply step_appR.
+    assumption.
+  - admit.
+Admitted.
+
 (* Strengthen IH for red_beta*)
-Lemma red_beta_ren x s t1 t2 rho : step t1 t2 -> red ([x := t1] (mren rho s)) ([x := t2] (mren rho s)).
+Lemma red_beta_ren x s t1 t2 rho : step t1 t2 -> { someAlpha : term & prod (red ([x := t1] (mren rho s)) someAlpha)
+            (Alpha [] someAlpha ([x := t2] (mren rho s))) }.
 Proof.
   elim: s rho t1 t2 => [Y|Y K1 T_body IH|T1 IH1 T2 IH2] rho t1 t2 Hstep.
   - unfold mren.
@@ -378,76 +1300,162 @@ Proof.
       * rewrite e.
         unfold lookup.
         rewrite eqb_refl.
-        apply star1.
-        assumption.
+        (* apply star1. *)
+        (* assumption. *)
+        admit.
       * unfold lookup.
-        destruct (x =? s).
-        -- apply star1.
+        destruct (x =? s);
+        admit.
+        (* -- apply star1.
            assumption.
-        -- apply starR.
+        -- apply starR. *)
     + destruct (string_dec x Y).
       * rewrite e.
         unfold lookup.
         rewrite eqb_refl.
-        apply star1.
-        assumption.
+        admit.
+        (* apply star1.
+        assumption. *)
       * unfold lookup.
-        destruct (x =? Y).
-        -- apply star1.
+        destruct (x =? Y);
+        admit.
+        (* -- apply star1.
            assumption.
-        -- apply starR.
+        -- apply starR. *)
   - (* lambda abstraction *)
     simpl.
     rewrite capms_equation_2.
     rewrite capms_equation_2.
     simpl.
-    remember (fresh2 [(x, t1)] (mren (drop Y rho) T_body)) as x'.
-    remember (fresh2 [(x, t2)] (mren (drop Y rho) T_body)) as x2.
-    rewrite (step_preserves_fresh_sigma (mren (drop Y rho) T_body) x Hstep) in Heqx'.
-    rewrite <- Heqx2 in Heqx'.
-    rewrite <- Heqx'.
+    remember (fresh2 [(Y, tmvar Y);(x, t1)] (mren (drop Y rho) T_body)) as x'.
+    remember (fresh2 [(Y, tmvar Y);(x, t2)] (mren (drop Y rho) T_body)) as x2. (* x' and x2 only equal if we dont look at bound vars*)
     remember (drop Y rho) as rho'.
-    apply red_abs.
-    
-    assert (exists rho'', rename Y x' (mren rho' T_body) = mren rho'' T_body).
-    {
-      apply ren_comp.
-    }
-    destruct H as [rho'' H].
-    rewrite H.
-    
-    apply IH.
-    assumption.
+    specialize (IH ((Y, x')::rho') t1 t2 Hstep).
+    destruct IH as [someAlpha [HredAlpha Halpha] ].
+
+    (* exists (tmlam x' K1 someAlpha). *)
+    eexists.
+    split.
+
+    + apply red_abs.
+
+      (* What if Y is in the RHS of rho' ?*)
+      assert (HrenComp: rename Y x' (mren rho' T_body) = mren ((Y, x')::rho') T_body).
+      {
+        admit.
+      }
+      rewrite HrenComp.
+      exact HredAlpha. 
+    + apply alpha_lam.
+
+      admit.
   - rewrite capms_equation_3.
     rewrite capms_equation_3.
-    apply red_app.
+    (* apply red_app.
     + apply IH1.
       assumption.
     + apply IH2.
-      assumption.
-Qed.
+      assumption.  *)
+Admitted.
 
 Lemma red_beta x s t1 t2 : step t1 t2 -> red ([x := t1] s) ([x := t2] s).
 Proof. 
-  move=> h. 
+  intros Hstep.
+  induction s.
+  - admit.
+  - rewrite capms_equation_2. simpl.
+    rewrite capms_equation_2. simpl.
+    remember (fresh2 [(x, t1)] s0) as s0'.
+    remember (fresh2 [(x, t2)] s0) as s0''.
+    (* apply red_abs. *)
+    
+  (* move=> h. 
   apply red_beta_ren with (rho := nil) (x := x) (s := s) in h.
-  rewrite mren_id in h.
-  assumption.
-Qed.
+  rewrite mren_id in h. *)
+  (* assumption. *)
+Admitted.
 
 (* Strong Normalization *)
 
-Notation SN := (sn step).
+(* used to be prop *)
+Inductive sn {e : term -> term -> Set } x : Set :=
+| SNI : (forall y, e x y -> sn y) -> sn x.
 
-Lemma sn_closed t s : SN (tmapp s t) -> SN s.
+(*
+Intuition:
+h x is strongly normalizing.
+then every reduction sequence starting from (h x) is finite.
+The first condition (e x y -> e (h x) (h y)) says that each step has a corresponding step under h.
+So in extension, each reduction chain starting from x has a corresponding reduction chain starting from h x.
+
+So, since h x is SN, every reduction chain starting from h x is finite.
+Then, by the extension, every reduction chain starting from x is finite.
+*)
+Lemma sn_preimage {e : term -> term -> Set} (h : term -> term) x :
+  (forall x y, e x y -> e (h x) (h y)) -> @sn e (h x) -> @sn e x.
+Proof.
+
+  move eqn:(h x) => v A B.
+  generalize dependent h.
+  generalize dependent x.
+  elim: B => {} v _ ih x h eqn.
+  intros A.
+  apply: SNI => y /A.
+  
+
+  
+  rewrite eqn => /ih. eauto.
+  Qed.
+
+Lemma sn_preimage_alpha {e : term -> term -> Set} (h : term -> term) x :
+  (forall x y, e x y -> { a : term & prod(Alpha [] (h y) a) (e (h x) a) }) -> 
+  @sn e (h x) -> { a2 : term & prod(Alpha [] x a2) (@sn e a2)}.
+Proof.
+  (* move eqn:(h x) => v A B. elim: B h x A eqn => {} v _ ih h x A eqn.
+  eexists.
+  split.
+  - admit.
+  - 
+  apply: SNI => y /A. rewrite eqn => /ih. apply/ih; eauto. *)
+Admitted.
+
+Notation SN := (@sn step).
+
+Lemma sn_closedL t s : SN (tmapp s t) -> SN s.
 Proof. apply: (sn_preimage (h := tmapp^~t)) => x y. exact: step_appL. Qed.
 
 Lemma sn_subst sigma s : SN (sigma [[s]]) -> SN s.
-Proof. apply: sn_preimage => x' y'. intros Hstep. exact: step_subst. Qed.
+Proof.
+Admitted.
+
+(* Not sure yet how to use the step_subst lemma in this*)
+Lemma sn_subst_alpha sigma s : SN (sigma [[s]]) -> {alphaS & prod (Alpha [] alphaS s) (SN alphaS)}.
+Proof.
+  (* intros H.
+  apply sn_preimage_alpha in H. 
+    - destruct H as [alphaS [Halpha Hsn] ].
+    exists alphaS.
+      split.
+      + eapply alpha_sym.
+        * constructor.
+        * assumption.
+      + assumption.
+    - intros x y Hstep.
+      apply (@step_subst_sigma x y sigma) in Hstep.
+      destruct Hstep as [alphaSigmaT [Hred Halpha] ].
+      exists alphaSigmaT.
+      split.
+      * eapply alpha_sym.
+        -- constructor.
+        -- assumption.
+      * assumption. *)
+Admitted.
+
+
 
 (* The Reducibility Candidates/Logical Predicate*)
 
-Definition cand := term -> Prop.
+Definition cand := term -> Set.
 
 Definition neutral (s : term) : bool :=
   match s with
@@ -455,12 +1463,14 @@ Definition neutral (s : term) : bool :=
     | _ => true
   end.
 
-Record reducible (P : cand) : Prop := {
+Record reducible (P : cand) : Set := {
   p_sn : forall s, P s -> SN s;
   p_cl : forall s t, P s -> step s t -> P t;
   p_nc : forall s, neutral s -> (forall t, step s t -> P t) -> P s
 }.
 
+(* **** The logical relation for proving Strong normalization, 
+        strengthens the IH to say something about labmda bodies*)
 Fixpoint L (T : type) : cand :=
   match T with
     | tp_base => SN 
@@ -470,9 +1480,9 @@ Fixpoint L (T : type) : cand :=
 (* TODO: Compare with Inductive instantiation from normalisation in
   PLF: that has a cleaner definition, but restraints the order*)
 Definition EL (Gamma : list (string * type)) 
-          (sigma : list (string * term)) : Prop :=
+          (sigma : list (string * term)) : Set :=
   forall x T, lookup x Gamma = Some T ->
-    exists t, lookup x sigma = Some t /\ L T t.
+    { t & prod (lookup x sigma = Some t) (L T t)}.
 
 (* is true! *)
 Lemma extend_EL (Gamma : list (string * type)) (sigma : list (string * term)) x T t :
@@ -483,7 +1493,15 @@ Admitted.
 (* Facts about reducible sets. *)
 
 Lemma reducible_sn : reducible SN.
-Proof. constructor; eauto using ARS.sn. by move=> s t [f] /f. Qed.
+Proof. 
+  constructor; eauto using ARS.sn. by move=> s t [f] /f. 
+
+  (*
+  
+  TODO INCOMPLETE
+  
+  *)
+Admitted.
 Global Hint Resolve reducible_sn : core.
 
 Lemma reducible_var P x : reducible P -> P (tmvar x).
@@ -495,7 +1513,7 @@ Proof with eauto using step.
   elim: A => /=[|A ih1 B ih2].
   - apply reducible_sn.
   - constructor.
-    + move=> s h. apply: (@sn_closed (tmvar "x")). apply: (p_sn (P := L B))...
+    + move=> s h. apply: (@sn_closedL (tmvar "x")). apply: (p_sn (P := L B))...
       eapply h. eapply reducible_var; eauto.
     + move=> s t h st u la. apply: (p_cl _ (s := tmapp s u))...
     + move=> s ns h t la.
@@ -546,15 +1564,15 @@ Proof with eauto.
   move=> snt h. have sns := sn_subst (L_sn h).
   elim: sns t snt h => {} s sns ih1 t. elim=> {} t snt ih2 h.
   apply: L_nc => // u st. inv st => //.
-  - inv H2. apply: ih1 => //. apply: L_cl h _. exact: step_subst.
+  - inv H2. apply: ih1 => //. apply: L_cl h _. admit. (* exact: step_subst. *) (* need to alphafy this lemma *)
   - apply: ih2 => //. apply: L_cl_star h _. exact: red_beta.
-Qed.
+Admitted.
 
 Lemma beta_expansion_subst X t sigma s A B :
   SN t -> L A (((X, t)::sigma) [[s]]) -> L A (tmapp (sigma [[tmlam X B s]]) t).
 Proof.
   intros snt H.
-  remember (fresh2 sigma s) as X'.
+  remember (fresh2 ((X, tmvar X)::sigma) s) as X'.
   assert (L A ([X' := t] (sigma [[(rename X X' s)]])) -> L A (tmapp (tmlam X' B (sigma [[rename X X' s]])) t)).
   {
     apply beta_expansion; assumption.
@@ -573,8 +1591,24 @@ Proof.
   - rewrite capmsRename.
     assumption.
   - rewrite -> HeqX'.
-    apply freshLemma.
-Qed.
+    (* apply freshLemma. easy by freshness*)
+    shelve.
+Admitted.
+
+(** Kinding of types *)
+Reserved Notation "Δ '|-*' T ':' K" (at level 40, T at level 0, K at level 0).
+Inductive has_type : list (string * type) -> term -> type -> Set :=
+  | K_Var : forall Δ X K,
+      List.lookup X Δ = Some K ->
+      Δ |-* (tmvar X) : K
+  | K_Lam : forall Δ X K1 T K2,
+      ((X, K1) :: Δ) |-* T : K2 ->
+      Δ |-* (tmlam X K1 T) : (tp_arrow K1 K2)
+  | K_App : forall Δ T1 T2 K1 K2,
+      Δ |-* T1 : (tp_arrow K1 K2) ->
+      Δ |-* T2 : K1 ->
+      Δ |-* (tmapp T1 T2) : K2
+where "Δ '|-*' T ':' K" := (has_type Δ T K).
 
 (* The fundamental theorem. *)
 Theorem soundness Gamma s A :
@@ -596,19 +1630,283 @@ Proof with eauto using L_sn.
     unfold L in ih1. fold L in ih1. specialize (ih1 (sigma [[t]]) ih2).
     rewrite capms_equation_3.
     assumption.
-Qed.
-
-Corollary type_L E s T : has_type E s T -> L T s.
-Proof.
-  move=> ty. move: (@soundness E s T ty) => h.
-  admit. (* TODO: Create some sort of identity subsittution*)
 Admitted.
 
-Corollary strong_normalization E s T : has_type E s T -> SN s.
+(* Identity substitutions: Given a typing context E, give a list of term substitutions matching this E*)
+Fixpoint id_subst (E : list (string * type)) : list (string * term) :=
+  match E with
+  | nil => nil
+  | cons (x, A) E' => cons (x, tmvar x) (id_subst E')
+  end.
+
+
+
+(* The identity substitution is in the EL relation *)
+
+Lemma id_subst_EL :
+  forall (E : list (string * type)),  EL E (id_subst E).
 Proof.
-  move=>/type_L/L_sn. apply.
+Admitted.
+
+(* TODO id_ren E could just be []? *)
+Lemma id_subst_alpha_type E s T :
+  has_type E s T -> Alpha [] s ((id_subst E) [[s]]).
+Proof.
+Admitted.
+
+(* The fundamental theorem for named variables. *)
+Corollary type_L (E : list (string * type)) s T : has_type E s T -> L T (id_subst E [[s]]).
+Proof.
+  intros Htype.
+  assert (HEL: EL E (id_subst E)) by apply id_subst_EL.
+  assert (Hsound: L T ((id_subst E) [[s]])) by apply (soundness Htype HEL).
+  assumption.
 Qed.
+
+Corollary strong_normalization_alpha E s T : has_type E s T -> SN (id_subst E [[s]]).
+Proof.
+  intros Hty.
+  apply type_L in Hty.
+  apply L_sn in Hty.
+  assumption.
+Qed.
+
+(* Monad maybe*)
+(* Define the bind function for option type *)
+Definition bind {A B : Type} (xx : option A) (f : A -> option B) : option B :=
+  match xx with
+  | None => None
+  | Some a => f a
+  end.
+
+Fixpoint is_normal (t : term) : bool :=
+  match t with
+  | tmlam X K T => is_normal T
+  | tmvar X => true
+  | tmapp T1 T2 => is_neutral T1 && is_normal T2
+  end
+
+with is_neutral (t : term) : bool :=
+  match t with
+  | tmvar X => true
+  | tmapp T1 T2 => is_neutral T1 && is_normal T2
+  | _ => false
+  end.
+
+  (** Normal types *)
+Inductive normal_Ty : term -> Prop :=
+  | NO_TyLam : forall x K T,
+      normal_Ty T ->
+      normal_Ty (tmlam x K T)
+  | NO_neutral : forall T,
+      neutral_Ty T ->
+      normal_Ty T
+
+with neutral_Ty : term -> Prop :=
+  | NE_TyVar : forall X,
+      neutral_Ty (tmvar X)
+  | NE_TyApp : forall T1 T2,
+      neutral_Ty T1 ->
+      normal_Ty T2 ->
+      neutral_Ty (tmapp T1 T2).
+
+(* Define an infix operator for bind *)
+Infix ">>=" := bind (at level 50, left associativity).
+
+(* Deterministic step *)
+Fixpoint step_d_f (t : term) : option term :=
+    match t with
+    | tmvar i => None
+    | tmapp s t => 
+        if is_normal s then
+            if is_normal t then
+                match s with
+                | tmlam x A s' => Some ([x := t] s')
+                | _ => None
+                end
+            else step_d_f t >>= fun t' => Some (tmapp s t')
+        else step_d_f s >>= fun s' => Some (tmapp s' t)
+    | tmlam x A s => (* step' s >>= _ does the normality check for us implicitly*)
+        step_d_f s >>= fun s' => Some (tmlam x A s')
+    end.
+
+Inductive step_d : term -> term -> Set :=
+| step_beta_d (x : string) (A : type) (s t : term) :
+    normal_Ty s ->
+    normal_Ty t ->
+    step_d (tmapp (tmlam x A s) t) ([x := t] s)
+| step_appL_d s1 s2 t :
+    step_d s1 s2 -> step_d (tmapp s1 t) (tmapp s2 t)
+| step_appR_d s t1 t2 :
+    normal_Ty s ->
+    step_d t1 t2 -> step_d (tmapp s t1) (tmapp s t2)
+| step_abs_d x A s1 s2 :
+    step_d s1 s2 -> step_d (tmlam x A s1) (tmlam x A s2).
+
+
+(* step_nd is a subset of step
+This is not true since step_d should use a different kind of substitution (only freshening when necessary)
+*)
+Lemma step_d_implies_step t t' : step_d t t' -> step t t'.
+Proof.
+  (* elim=> H; constructor; try assumption. *)
+Abort.
+
+Lemma step_d_implies_step_alpha t t' : step_d t t' -> { t'_alpha : term & prod(Alpha [] t' t'_alpha) (step t t'_alpha)}.
+Proof.
+  intros Hstep.
+  induction Hstep.
+  - (* this is proving that if substituteTCA x t s is alpha to [x := t] s (capmsfr)*) admit.
+  - admit.
+  - admit.
+  - destruct IHHstep as [IHHt' [IHHalpha IHHstep'] ].
+    exists (tmlam x A IHHt').
+    split.
+    + apply alpha_lam.
+      apply alpha_extend_id'.
+      * assumption.
+      * apply not_break_shadow_nil.
+    + apply step_abs.
+      assumption.
+Admitted.
+
+(* Does this still work now we no longer have step_d_implies_step?
+  Maybe if we make it up to alhpa
+ *)
+Lemma SN_d : forall t, (@sn step) t -> {t_alpha : term & prod (Alpha [] t t_alpha) ((@sn step_d) t_alpha)}.
+Proof.
+  intros t HSN.
+  induction HSN.
+  eexists.
+  split.
+  - admit.
+  - (* oof. I dont know how to prove this. Maybe we need a weaker SN notion or something:
+    @sn step_d x -> exists z, Alpha [] x z AND forall y, step z y -> SN y
+   *)
+Admitted.
+
+(* Main lemma for going from using t alpha t' in SN t' to SN t*)
+Lemma step_preserves_alpha_d sigma s t s' t' :
+  Alpha sigma s t -> step_d s s' -> step_d t t' -> Alpha sigma s' t'.
+Proof.
+Admitted.
+
+Require Import Coq.Program.Equality.
+
+(*I do not like these lemmas. Maybe we can change the definition of normality to equal not being able to step? *)
+Lemma is_normal_no_step_d t :
+  is_normal t = true -> step_d_f t = None.
+Proof.
+Admitted.
+
+Lemma is_normal_then_step_d t :
+  is_normal t = false -> ~ step_d_f t = None.
+Proof.
+Admitted.
+
+(* We also need this for sound/completeness, so we can assume it is true/a good approach*)
+Lemma is_normal_then_normal_Ty t : 
+  is_normal t = true -> normal_Ty t.
+Proof.
+Admitted.
+
+
+Lemma step_d_f_to_step_d : forall t t', step_d_f t = Some t' -> step_d t t'.
+Proof.
+  intros t t' Hstep_d_f.
+  dependent induction t. (* we needed IH over t' *)
+  - discriminate.
+  - destruct (is_normal t0) eqn: Hnormal_s.
+    + apply is_normal_no_step_d in Hnormal_s.
+      inversion Hstep_d_f.
+      rewrite Hnormal_s in H0.
+      inversion H0.
+      (* If t0 is normal, then also tmlam s t t0*)
+    + destruct (step_d_f t0) eqn: Hstep_t.
+      * inversion Hstep_d_f.
+        rewrite Hstep_t in H0.
+        inversion H0.
+        apply step_abs_d.
+        specialize (IHt t1).
+        apply IHt.
+        reflexivity.
+      * apply is_normal_then_step_d in Hnormal_s.
+        contradiction.
+  - inversion Hstep_d_f.
+    destruct (is_normal t1) eqn: Hnormal_s.
+    + destruct (is_normal t2) eqn: Hnormal_t.
+      * destruct t1. (* case step_beta *)
+        -- discriminate.
+        -- inversion Hnormal_s.
+           inversion Hnormal_t.
+           inversion H0.
+           apply step_beta_d.
+           ++ apply is_normal_then_normal_Ty.
+              assumption. (* is_normal -> normal_ty, we need that anyway for sound/completeness*)
+           ++ apply is_normal_then_normal_Ty.
+              assumption.
+        -- discriminate.
+      * destruct (step_d_f t2) eqn: Hstep_t. (* IH was not strong enough, so dependent induction *)
+        -- inversion H0.
+           apply step_appR_d.
+           ++ apply is_normal_then_normal_Ty.
+              assumption.
+           ++ apply IHt2. 
+              reflexivity.
+        -- discriminate.
+    + destruct (step_d_f t1) eqn: Hstep_s.
+      * inversion H0.
+        apply step_appL_d.
+        apply IHt1.
+        reflexivity.
+      * discriminate.
+Qed.
+
+(* eq_refl didnt work, this does, thank Copilot, but I dont understand *)
+Lemma eq_proof {A : Type} (x : A) : x = x.
+Proof. reflexivity. Qed.
+
+(* Terminating normalization procedure helper.
+  We can normalize a term given that we know that an 
+  alpha equivalent term is strongly normalizing
+*)
+Fixpoint normalizer' {sigma : list (string * string)} (t t' : term) (HAlpha : Alpha sigma t t') (HSN : (@sn step_d) t') : term :=
+  match step_d_f t as res return (step_d_f t = res -> term) with
+  | None => fun _ => t
+  | Some t1 => fun Hstep =>
+      match step_d_f t' as res' return (step_d_f t' = res' -> term) with
+      | None => fun _ => t1 (* Uhm. Cannot happen. How to show this to coq? *)
+      | Some t'1 => fun Hstep' =>
+          let HStep_d := step_d_f_to_step_d Hstep in
+          let HStep_d' := step_d_f_to_step_d Hstep' in
+          let HAlpha' := step_preserves_alpha_d HAlpha HStep_d HStep_d' in
+          let HSN' := match HSN with
+                      | SNI f => f t'1 HStep_d'
+                      end in
+          @normalizer' sigma t1 t'1 HAlpha' HSN'
+      end (eq_proof (step_d_f t'))
+  end (eq_proof (step_d_f t)).
+
+(* Normalization procedure for well typed terms *)
+Definition normalizer E T (t : term) (Htype : has_type E t T) : term :=
+  let t' := id_subst E [[t]] in
+  let HAlpha := @id_subst_alpha_type E t T Htype in
+  let HSN := strong_normalization_alpha Htype in
+  let (t'', p ) := SN_d HSN in
+  let (HAlpha', SNstep_d_t'') := p in
+
+    (* HAlpha says Alpha [] t t'
+       HAlpha' says Alpha [] t' t''
+       
+    Hence by transitivity: Alpha [] t t''
+    *)
+  let HAlphaTrans := alpha_trans alpha_trans_nil HAlpha HAlpha' in
+      @normalizer' [] t t'' HAlphaTrans SNstep_d_t''.
+
 
 (* Local Variables: *)
 (* coq-load-path: (("." "Ssr")) *)
 (* End: *)
+
+
+*)
